# GPT Prompt 1: Formalize Theorem D.1 (Algebraic Equivalence)

## Task

Formalize Dyachenko's Theorem D.1, which establishes the equivalence between the "product identity" form and the "sum condition" form of the ED2 equation.

## Mathematical Statement

**Theorem D.1.** Let alpha, b', c', P be positive natural numbers with A := alpha * b' * c' and m := 4*A - P > 0. The following are equivalent:

1. There exists d' in N+ such that:
   (4*alpha*d'*b' - 1) * (4*alpha*d'*c' - 1) = 4*alpha*P*d'^2 + 1

2. m divides (b' + c')

Moreover, when these hold, d' = (b' + c') / m.

## Proof Sketch

Expand the LHS of (1):
```
(4*alpha*d'*b' - 1) * (4*alpha*d'*c' - 1)
= 16*alpha^2*d'^2*b'*c' - 4*alpha*d'*b' - 4*alpha*d'*c' + 1
= 16*alpha^2*d'^2*b'*c' - 4*alpha*d'*(b' + c') + 1
```

Set this equal to RHS = 4*alpha*P*d'^2 + 1:
```
16*alpha^2*d'^2*b'*c' - 4*alpha*d'*(b' + c') + 1 = 4*alpha*P*d'^2 + 1
```

Cancel the +1:
```
16*alpha^2*d'^2*b'*c' - 4*alpha*d'*(b' + c') = 4*alpha*P*d'^2
```

Divide by 4*alpha*d' (positive, so safe):
```
4*alpha*d'*b'*c' - (b' + c') = P*d'
```

Since A = alpha*b'*c', we have 4*alpha*b'*c' = 4*A:
```
4*A*d' - (b' + c') = P*d'
d' * (4*A - P) = b' + c'
d' * m = b' + c'
```

Hence m | (b' + c') and d' = (b' + c') / m.

## Lean Statement to Prove

```lean
import Mathlib.Tactic

namespace ED2

/-- Theorem D.1: The product identity is equivalent to the sum divisibility condition. -/
theorem d1_product_sum_equiv
    {alpha b' c' P : ℕ}
    (halpha : 0 < alpha) (hb : 0 < b') (hc : 0 < c') (hP : 0 < P)
    (hm : P < 4 * alpha * b' * c')  -- ensures m = 4A - P > 0
    : let A := alpha * b' * c'
      let m := 4 * A - P
      (∃ d' : ℕ, 0 < d' ∧
        (4 * alpha * d' * b' - 1) * (4 * alpha * d' * c' - 1) = 4 * alpha * P * d' ^ 2 + 1)
      ↔
      (m ∣ (b' + c')) := by
  sorry

/-- When the conditions hold, d' is uniquely determined. -/
theorem d1_d'_formula
    {alpha b' c' P d' : ℕ}
    (halpha : 0 < alpha) (hb : 0 < b') (hc : 0 < c') (hP : 0 < P) (hd' : 0 < d')
    (hm : P < 4 * alpha * b' * c')
    (hprod : (4 * alpha * d' * b' - 1) * (4 * alpha * d' * c' - 1) = 4 * alpha * P * d' ^ 2 + 1)
    : let A := alpha * b' * c'
      let m := 4 * A - P
      d' = (b' + c') / m := by
  sorry

end ED2
```

## Hints

1. Work in ℤ to avoid Nat subtraction issues, then cast back.
2. The expansion and simplification is mostly `ring` and `nlinarith`.
3. For the division, use `Nat.div_mul_cancel` once you've shown divisibility.
4. The key insight: 4*A = 4*alpha*b'*c', so the algebra simplifies nicely.

## What NOT to do

- Don't use sorry in the final proof
- Don't import anything beyond Mathlib.Tactic (it's sufficient)
- Don't worry about connecting this to other theorems yet - just prove D.1 in isolation

## Deliverable

Provide complete Lean 4 proofs for both theorems above.
